src/ocamlmm/OCamlToimm_s_prog_build_graph.v
@@ -1,0 +1,515 @@
+(******************************************************************************)
+(** * ocaml MM is weaker than IMM_S   *)
+(******************************************************************************)
+Require Import Classical Peano_dec.
+From hahn Require Import Hahn.
+Require Import Omega.
+Require Import Events.
+Require Import Execution.
+Require Import Execution_eco.
+Require Import imm_common.
+Require Import imm_s_hb.
+Require Import imm_s.
+Require Import OCaml.
+Require Import OCamlToimm_s.
+Require Import OCamlToimm_s_prog. 
+Require Import OCamlToimm_s_prog_compilation.
+Require Import OCamlToimm_s_prog_pair_step. 
+(* Require Import OCamlToimm_s_prog_bounded_properties.  *)
+(* Require Import OCamlToimm_s_compcorrhelpers.  *)
+Require Import OCamlToimm_s_steps. 
+Require Import Utils.
+Require Import ClosuresProperties. 
+Require Import Prog.
+Require Import ProgToExecution.
+Require Import ProgToExecutionProperties.
+Require Import Logic.Decidable. 
+From PromisingLib Require Import Basic Loc.
+Require Import Basics. 
+Set Implicit Arguments.
+
+  
+Section BUILD_OMM_GRAPH.
+
+  Lemma thread_execs tid PO PI (COMP: is_thread_compiled PO PI)
+        SGI (ExI: thread_execution tid PI SGI):
+    exists SGO, Othread_execution tid PO SGO /\
+           same_behavior_local SGO SGI. 
+  Proof.
+    red in ExI. destruct ExI as [sti_fin ExI]. desc.
+    apply (@crt_num_steps _ (step tid) (init PI) sti_fin) in STEPS as [n_isteps ISTEPS].
+    assert (SAME_INSTRS: PI = instrs sti_fin). 
+    { replace PI with (instrs (init PI)); auto. 
+      apply steps_same_instrs. exists tid. apply <- crt_num_steps. eauto. }
+    red in COMP. desc.
+    set (bsti_fin := {|
+          binstrs := BPI;
+          bpc := length BPI;
+          bG := G sti_fin;
+          beindex := eindex sti_fin;
+          bregf := regf sti_fin;
+          bdepf := depf sti_fin;
+          bectrl := ectrl sti_fin |}). 
+    assert (sti_fin = bst2st bsti_fin) as BST. 
+    { unfold bst2st. 
+      simpl.
+      rewrite firstn_all.
+      red in COMP. desc.
+      rewrite <- COMP0.
+      rewrite SAME_INSTRS.
+      apply is_terminal_pc_bounded in TERMINAL. 
+      rewrite <- TERMINAL; auto.
+      (* TODO: why so complicated? *)      
+      apply state_record_equality. } 
+    
+    assert (is_block_terminal bsti_fin) as BLOCK_TERM. 
+    { red. destruct (dec_ge (bpc bsti_fin) (length (binstrs bsti_fin))); auto. }
+    assert (exists n_osteps, (omm_block_step tid) ^^ n_osteps (binit BPI) bsti_fin) as [n_osteps OMM_STEPS]. 
+    { apply crt_num_steps.
+      forward eapply (@steps_imply_ommblocks bsti_fin _ tid); eauto.
+      { exists PO. red in COMP. desc. auto. }
+      Unshelve. 2: simpl; omega. 
+      rewrite <- BST. apply crt_num_steps.
+      rewrite <- SAME_INSTRS. eauto. }
+    
+    assert (BY_STEPS:
+              forall i bsti_i (INDEX: i <= n_osteps)
+                (STEPS_TO: (omm_block_step tid)^^i (binit BPI) bsti_i)
+                (STEPS_FROM: (omm_block_step tid)^^(n_osteps - i) bsti_i bsti_fin),
+                 exists sto_i,
+                 (Ostep tid)^^i (init PO) sto_i /\
+                 mm_similar_states sto_i bsti_i /\
+                 pc sto_i <= length PO).
+    { induction i.
+      - intros bsti_i _ STEPS_TO STEPS_FROM.
+        exists (init PO). splits; [basic_solver| | simpl; omega].
+        replace (bsti_i) with (binit BPI); [apply init_mm_same; auto| ].
+        { red in COMP. desc. auto. }
+        generalize STEPS_TO. simpl. basic_solver 10.
+      - intros bsti_i INDEX STEPS_TO STEPS_FROM.
+        rewrite step_prev in STEPS_TO.
+        destruct STEPS_TO as [bsti_i' [STEPS_TO' STEPS_FROM']].
+        forward eapply IHi as [sto' [OSTEPS' [MM_SIM' PCO_BOUND]]]. 
+        { omega. }
+        { eauto. }
+        { apply (@steps_split _ _ _ 1 (n_osteps - S i)); [omega| ].
+          eexists. split; eauto. simpl. basic_solver. }
+
+        forward eapply (@clos_refl_trans_mori _ (omm_block_step tid) (block_step tid)).
+        { red. ins. apply bs_extract. auto. }
+        intros OB_B.
+        assert (bpc bsti_i <= length (binstrs bsti_i')) as BPC_BOUND.
+        { replace (binstrs bsti_i') with (binstrs bsti_i).
+          2: { red in STEPS_FROM'. desc. auto. }
+          destruct (gt_0_eq (n_osteps - S i)) as [GT | FIN].
+          2: { rewrite <- FIN in STEPS_FROM.
+               apply (steps0 (omm_block_step tid)) in STEPS_FROM.
+               subst bsti_i. auto. }
+          apply Nat.lt_le_incl. apply nth_error_Some, OPT_VAL. 
+          apply steps_sub with (m := 1) in STEPS_FROM; [| omega].
+          destruct STEPS_FROM as [bst_next STEP_NEXT].
+          apply (same_relation_exp (pow_unit (omm_block_step tid))) in STEP_NEXT. 
+          red in STEP_NEXT. desc. red in BLOCK_STEP. desc. eauto. }          
+        assert (bpc bsti_i' <= length (binstrs bsti_i')).
+        { red in MM_SIM'. desc. rewrite <- MM_SIM'0.
+          replace (length (binstrs bsti_i')) with (length PO); auto.
+          apply compilation_same_length.
+          replace PO with (instrs sto'); auto.
+          replace PO with (instrs (init PO)) by vauto.
+          symmetry. apply omm_steps_same_instrs. exists tid. apply <- crt_num_steps. eauto. }
+        assert (SAME_BINSTRS': BPI = binstrs bsti_i').
+        { replace BPI with (binstrs bsti_fin); auto. symmetry. 
+          apply (@inclusion_t_ind _ (block_step tid) (fun x y => binstrs x = binstrs y)).
+          { red. ins. eapply SAME_BINSTRS. eauto. }
+          { red. ins. congruence. }
+          apply t_step_rt. exists bsti_i. split.
+          { apply bs_extract. auto. }
+          apply OB_B. apply crt_num_steps. eexists. eauto. }
+
+        forward eapply (pair_step MM_SIM' STEPS_FROM') as [sto [OSTEP MM_SIM]]; eauto. 
+        { apply OB_B. apply crt_num_steps. exists i.
+          replace (binstrs bsti_i') with BPI; auto. }
+        exists sto. splits; eauto.
+        2: { red in MM_SIM. desc.
+             replace (length PO) with (length (binstrs bsti_i')); [omega|].
+             replace (binstrs bsti_i') with BPI; auto.
+             symmetry. apply compilation_same_length.
+             red in COMP. desc. auto. }
+        apply step_prev. eexists. splits; eauto. }
+    
+    forward eapply (BY_STEPS n_osteps bsti_fin (Nat.le_refl n_osteps)) as [sto_fin [OSTEPS [MM_SIM PC_BOUND]]].
+    { auto. }
+    { rewrite Nat.sub_diag. basic_solver. }
+    assert (SAME_OINSTRS: PO = instrs sto_fin).
+    { replace PO with (instrs (init PO)); auto.
+      apply omm_steps_same_instrs. exists tid. apply <- crt_num_steps. eauto. }
+    
+    exists (G sto_fin).
+    splits.
+    { red. exists sto_fin. splits; auto. 
+      { apply crt_num_steps. vauto. }
+      apply is_terminal_new.
+      replace (length (instrs sto_fin)) with (length (binstrs bsti_fin)).
+      2: { symmetry. apply compilation_same_length. rewrite <- SAME_OINSTRS.
+           subst bsti_fin. simpl. red in COMP. desc. auto. }
+      replace (pc sto_fin) with (bpc bsti_fin).
+      2: { red in MM_SIM. desc. auto. }
+      apply BLOCK_TERM. }
+    { red in MM_SIM. desc.
+      replace SGI with (bG bsti_fin); auto. }
+  Qed.
+
+
+
+  Variable ProgO ProgI: Prog.Prog.t.
+  Hypothesis Compiled: is_compiled ProgO ProgI.
+  Hypothesis OCamlProgO: OCamlProgram ProgO.
+  
+  Variable GI: execution.
+  Hypothesis WFI: Wf GI.
+  Variable sc: relation actid. 
+  Hypothesis ExecI: program_execution ProgI GI.
+  Hypothesis IPC: imm_s.imm_psc_consistent GI sc.
+
+  Hypothesis programs_without_tid_init: ~ (IdentMap.In tid_init ProgI).
+
+  Notation "'E' G" := G.(acts_set) (at level 1).
+  Notation "'R' G" := (fun a => is_true (is_r G.(lab) a)) (at level 1).
+  Notation "'W' G" := (fun a => is_true (is_w G.(lab) a)) (at level 1).
+  Notation "'RW' G" := (R G ∪₁ W G) (at level 1).  
+  Notation "'F' G" := (fun a => is_true (is_f G.(lab) a)) (at level 1).
+  Notation "'ORlx' G" := (fun a => is_true (is_only_rlx G.(lab) a)) (at level 1).
+  Notation "'Sc' G" := (fun a => is_true (is_sc G.(lab) a)) (at level 1). 
+  Notation "'Acq' G" := (fun a => is_true (is_acq G.(lab) a)) (at level 1). 
+  Notation "'Acqrel' G" := (fun a => is_true (is_acqrel G.(lab) a)) (at level 1). 
+  Notation "'R_ex' G" := (fun a => is_true (R_ex G.(lab) a)) (at level 1).
+  Notation "'hbo'" := (OCaml.hb). 
+  Notation "'same_loc' G" := (same_loc G.(lab)) (at level 1).
+  Notation "'Tid_' t" := (fun x => tid x = t) (at level 1).
+
+
+  Record hlpr := { htid: thread_id; hPO: list Instr.t; hPI: list Instr.t; hSGI: execution}.
+  
+  Definition hlpr_restr hlpr := 
+    ⟪THREADO': Some (hPO hlpr) = IdentMap.find (htid hlpr) ProgO ⟫/\
+    ⟪THREADI': Some (hPI hlpr) = IdentMap.find (htid hlpr) ProgI ⟫ /\
+    ⟪RESTR': thread_restricted_execution GI (htid hlpr) (hSGI hlpr) ⟫. 
+    
+  Definition hlpr_GO SGO hlpr :=
+    ⟪OEXEC':Othread_execution (htid hlpr) (hPO hlpr) SGO ⟫ /\
+    ⟪SBL': same_behavior_local SGO (hSGI hlpr) ⟫.
+
+  Definition intra_E G :=
+    rmw G ≡ ⦗E G⦘ ⨾ rmw G ⨾ ⦗E G⦘ /\
+    data G ≡ ⦗E G⦘ ⨾ data G ⨾ ⦗E G⦘ /\
+    ctrl G ≡ ⦗E G⦘ ⨾ ctrl G ⨾ ⦗E G⦘ /\
+    addr G ≡ ⦗E G⦘ ⨾ addr G ⨾ ⦗E G⦘ /\
+    rmw_dep G ≡ ⦗E G⦘ ⨾ rmw_dep G ⨾ ⦗E G⦘. 
+
+  
+  Lemma sbl_sim_rect GI1 GO1 GI2 GO2 (SIM: graphs_sim_weak GI1 GI2)
+        (SBL: same_behavior_local GO1 GI1)
+        (SBL': same_behavior_local GO2 GI2)
+        (INTRA_E: intra_E GI1):
+    graphs_sim_weak GO1 GO2.
+  Proof.
+    apply sbl_ext_TMP in SBL. apply sbl_ext_TMP in SBL'.
+    red in SIM, SBL, SBL'. desc.
+    assert (E GI1 ∩₁ RWO GI1 ≡₁ E GI1 ∩₁ RWO GI2) as E_RWO.
+    { unfold RWO. rewrite <- SIM1. repeat rewrite set_inter_minus_r.
+      apply set_equiv_inter; [| basic_solver].
+      apply inter_subset_helper. ins. unfold is_r, is_w, set_union.
+      rewrite SIM0; vauto. }
+    assert (forall rel (RESTR1: rel GO1 ≡ restr_rel (RWO GI1) (rel GI1))
+              (RESTR2: rel GO2 ≡ restr_rel (RWO GI2) (rel GI2))
+              (EQV: rel GI1 ≡ rel GI2)
+              (ON_E: rel GI1 ≡ ⦗E GI1⦘ ⨾ rel GI1 ⨾ ⦗E GI1⦘),
+               rel GO1 ≡ rel GO2) as INTRA_HELPER. 
+    { ins. rewrite RESTR1, RESTR2, <- EQV.
+      rewrite ON_E.
+      rewrite <- restr_relE. do 2 rewrite restr_restr.
+      apply restr_rel_more; [done | basic_solver]. }
+    assert (E GO1 ≡₁ E GO2) as E_EQ.
+    { rewrite RESTR_EVENTS, RESTR_EVENTS0. rewrite <- SIM. auto. }
+    red. splits; auto. 
+    { ins. assert (E GO2 x) as E2 by (apply E_EQ; auto). 
+      rewrite SAME_LAB, SAME_LAB0; auto.
+      apply SIM0. rewrite (set_equiv_exp RESTR_EVENTS0) in H.
+      red in H. desc. auto. }
+    all: red in INTRA_E; desc; intuition. 
+  Qed. 
+
+  Lemma wf_tre_intra_E G thread (WF: Wf G) Gi
+        (TRE: thread_restricted_execution G thread Gi):
+    intra_E Gi.
+  Proof. 
+    red. destruct TRE. 
+    assert (forall rel (THREAD_RESTR: rel Gi ≡ ⦗Tid_ thread⦘ ⨾ rel G ⨾ ⦗Tid_ thread⦘)
+              (REL_E: rel G ≡ ⦗E G⦘ ⨾ rel G ⨾ ⦗E G⦘),
+               rel Gi  ≡ ⦗E Gi⦘ ⨾ rel Gi ⨾ ⦗E Gi⦘) as E_HELPER. 
+    { ins. rewrite THREAD_RESTR, REL_E. 
+      rewrite <- !restr_relE, !restr_restr.
+      apply restr_rel_more; [| basic_solver].
+      rewrite tr_acts_set. basic_solver. } 
+    Hint Resolve wf_rmwE wf_dataE wf_addrE wf_ctrlE wf_rmw_depE. 
+    destruct WFI.
+    splits. all: apply E_HELPER; auto.
+  Qed.
+
+  Lemma sbl_sim GO1 GO2 G (SBL1: same_behavior_local GO1 G) (SBL2: graphs_sim_weak GO1 GO2):
+    same_behavior_local GO2 G.
+  Proof.
+    apply sbl_ext_TMP in SBL1.
+    cut (same_behavior_local_ext GO2 G).
+    { ins. red in H. desc. vauto. }
+    red in SBL1. red in SBL2. desc.
+    assert (forall (r1 r2: execution -> relation actid) R3 (EQ: r1 GO1 ≡ r2 GO2) (TGT: r1 GO1 ≡ R3), r2 GO2 ≡ R3) as TRANS by basic_solver.
+    red. splits.
+    all: try (by eapply TRANS; vauto).
+    { rewrite <- SBL2. auto. }
+    ins. rewrite <- (set_equiv_exp SBL2) in EGOx. 
+    rewrite <- SBL0; intuition.
+  Qed. 
+  
+    
+  Lemma tre_sim_weak G G1 G2 thread
+        (TRE1: thread_restricted_execution G thread G1)
+        (TRE2: thread_restricted_execution G thread G2):
+    graphs_sim_weak G1 G2. 
+  Proof.
+    destruct TRE1, TRE2. red.
+    assert (E G1 ≡₁ E G2) as E_EQV.
+    { symmetry in tr_acts_set0. eapply set_equiv_rel_Transitive; eauto. }
+    splits; auto.
+    { ins. rewrite tr_lab; auto. rewrite tr_lab0; auto. apply E_EQV. auto. }
+    all: eapply same_rel_Transitive; eauto; symmetry; auto. 
+  Qed. 
+    
+  
+  Lemma thread_execs_helper: exists GO,
+      ⟪ E_STRUCT: forall e : actid, E GO e -> is_init e \/ IdentMap.In (tid e) ProgO ⟫/\
+      ⟪ SAME_INIT: E GO ∩₁ is_init ≡₁ E GI ∩₁ is_init⟫ /\
+      ⟪ SAME_INIT_LABELS: forall l, lab GO (InitEvent l) = Astore Xpln Opln l 0 ⟫ /\
+      ⟪ SAME_CO: co GI ≡ co GO⟫ /\
+      ⟪ EXT_RF: rf GO ≡ restr_rel (RWO GI) (rf GI)⟫ /\
+      ⟪ RESTR_SIM: forall tid POi
+        (THREAD: Some POi = IdentMap.find tid ProgO)
+        GOi (RESTR: thread_restricted_execution GO tid GOi)
+        GIi (RESTR: thread_restricted_execution GI tid GIi),
+        Othread_execution_sim tid POi GOi /\ same_behavior_local GOi GIi ⟫.
+  Proof.
+    set (all_acts := set_bunion
+                       hlpr_restr
+                       (fun hlpr e => exists GOi, hlpr_GO GOi hlpr /\ E GOi e)).
+
+    set (GOi_prop := fun thread GOi =>
+                       exists POi GIi,
+                         Some POi = IdentMap.find thread ProgO /\
+                         thread_restricted_execution GI thread GIi /\
+                         Othread_execution thread POi GOi /\
+                         same_behavior_local GOi GIi).
+    
+    assert (set_finite all_acts) as FIN_EGO. 
+    { red. exists (acts GI). ins.
+      do 2 red in IN. destruct IN as [[tid POi PIi GIi] [HLPR_RESTR [GOi [HLPR_GO EGOx]]]].
+      cut (E GIi x).
+      { ins. red in HLPR_RESTR. desc. simpl in *.
+        destruct RESTR'. rewrite (set_equiv_exp tr_acts_set) in H.
+        red in H. desc. auto. }
+      red in HLPR_GO. desc. simpl in *.
+      red in SBL'. desc. rewrite (set_equiv_exp RESTR_EVENTS) in EGOx.
+      red in EGOx. desc. auto. }
+    apply set_finite_alt in FIN_EGO. destruct FIN_EGO as [GO_actsset EGO].
+    assert (set_finite (E GI ∩₁ is_init)) as FIN_INIT.
+    { red. exists (acts GI). ins. red in IN. desc. auto. }
+    apply set_finite_alt in FIN_INIT. destruct FIN_INIT as [GO_initset INIT_GO].
+    set (GOi_rel := fun (rel: execution -> relation actid) =>
+                      bunion
+                        hlpr_restr
+                        (fun hlpr x y => exists GOi, (hlpr_GO GOi hlpr) /\ (rel GOi x y))). 
+    set (GO :=   {| acts := GO_actsset ++ GO_initset;
+                    lab := lab GI;
+                    rmw := GOi_rel rmw; 
+                    data := GOi_rel data;
+                    addr := GOi_rel addr;
+                    ctrl := GOi_rel ctrl;
+                    rmw_dep := GOi_rel rmw_dep;
+                    rf := restr_rel (RWO GI) (rf GI);
+                    co := co GI |}).
+    assert (forall e (E_ACT: In e GO_actsset), exists thread index GOi,
+                 e = ThreadEvent thread index /\
+                 GOi_prop thread GOi) as E_GO_STRUCT.
+    { ins.
+      apply EGO in E_ACT. subst all_acts.
+      red in E_ACT. destruct E_ACT as [[thread' POi' PI' GI'] [THREAD [GOi [EGOi_prop EGOi]]]]. 
+      red in EGOi_prop. red in THREAD. desc. simpl in *. 
+      red in SBL'. desc. rewrite (set_equiv_exp RESTR_EVENTS) in EGOi.
+      red in EGOi. desc. 
+      destruct RESTR'. rewrite (set_equiv_exp tr_acts_set) in EGOi.
+      red in EGOi. desc.
+      destruct e.
+      { subst. exfalso. apply programs_without_tid_init.
+        apply find_iff_in. simpl in THREADI'. vauto. }
+      simpl in EGOi1. subst. do 3 eexists; eauto. split; eauto. vauto. }
+
+    exists GO. splits.
+    { subst GO. unfold acts_set. simpl. ins.
+      destruct e; [by vauto| ].
+      right. simpl.
+      apply in_app_or in H. des.
+      2: { apply INIT_GO in H. red in H. desc.
+           unfold is_init in H0. vauto. }
+      apply E_GO_STRUCT in H. desc. inversion H. subst.
+      red in H0. desc. apply find_iff_in. eauto. }
+    { subst GO. unfold acts_set. simpl.
+      assert (forall {A: Type} (l1 l2: list A), (fun x => In x (l1 ++ l2)) ≡₁ (fun x => In x l1) ∪₁ (fun x => In x l2)) as IN_SET_UNION.
+      { ins. apply set_equiv_exp_iff. ins. split.
+        { ins. red. apply in_app_or. auto. }
+        ins. red in H. apply in_or_app. auto. }
+      rewrite IN_SET_UNION, set_inter_union_l.
+      arewrite ((fun x : actid => In x GO_actsset) ∩₁ (fun a : actid => is_init a) ≡₁ ∅).
+      { split; [| basic_solver]. red. ins. red in H. desc.
+        apply E_GO_STRUCT in H. desc. subst. unfold is_init in H0. vauto. }
+      remove_emptiness. rewrite <- set_interK with (s := is_init) at 2.
+      rewrite <- set_interA. apply set_equiv_inter; [| basic_solver].
+      symmetry. apply set_equiv_exp_iff. apply INIT_GO. }
+    2: { vauto. }
+    2: { vauto. }
+    { simpl. destruct WFI. auto. }
+    ins.
+    assert (exists PIi, Some PIi = IdentMap.find tid ProgI) as [PIi THREADI].
+    { apply find_iff_in. red in Compiled. destruct Compiled. apply H.
+      apply find_iff_in. vauto. }
+    assert (is_thread_compiled POi PIi) as COMP.
+    { red in Compiled. destruct Compiled. red in H0. eapply H0; vauto. }
+    assert (thread_execution tid PIi GIi) as EXECIi. 
+    { apply program_execution_equiv in ExecI. destruct ExecI.
+      apply H0; auto. }
+    pose proof (thread_execs COMP EXECIi) as [SGO [OEXEC SBL]]. desc.
+    apply sbl_ext_TMP in SBL. 
+    cut (graphs_sim_weak SGO GOi).
+    { ins. split.
+      { red. red in OEXEC. desc.
+        exists s. splits; vauto. }
+      eapply sbl_sim; vauto.
+      red in SBL. desc. vauto. }
+    assert (forall rel
+              (RWO_RESTR_IF_SBL: forall Go Gi,
+                  same_behavior_local_ext Go Gi ->
+                  rel Go ≡ restr_rel (RWO Gi) (rel Gi))
+              (TID_RESTR_IF_TRE: forall G G' tid,
+                  thread_restricted_execution G tid G' ->
+                  rel G' ≡ ⦗Tid_ tid⦘ ⨾ rel G ⨾ ⦗Tid_ tid⦘)
+              (REL_GO: rel GO ≡ GOi_rel rel)
+              (REL_EQ_IF_GSW: forall GOi', graphs_sim_weak SGO GOi' -> rel SGO ≡ rel GOi'),
+               rel SGO ≡ rel GOi) as INTRA_REL_HELPER. 
+    { ins.
+      rewrite (RWO_RESTR_IF_SBL _ _ SBL).
+      rewrite (TID_RESTR_IF_TRE _ _ _ RESTR). rewrite REL_GO.  
+      unfold GOi_rel.
+      rewrite seq_bunion_l, seq_bunion_r.
+      apply same_relation_exp_iff. ins. split.
+      { intros [RELxy [RWOx RWOy]]. 
+        exists ({| htid := tid; hPO := POi; hPI := PIi; hSGI := GIi |}).
+        splits; vauto. apply seq_eqv_lr.
+        rewrite (same_relation_exp (TID_RESTR_IF_TRE _ _ _ RESTR0)) in RELxy.
+        apply seq_eqv_lr in RELxy. desc.
+        splits; vauto. 
+        exists SGO. splits.
+        { unfold hlpr_GO. simpl. destruct SBL. desc. splits; vauto. }
+        rewrite (same_relation_exp (RWO_RESTR_IF_SBL _ _ SBL)).
+        red. splits; auto.
+        rewrite (same_relation_exp (TID_RESTR_IF_TRE _ _ _ RESTR0)). 
+        apply seq_eqv_lr. splits; auto. }
+      { ins. red in H. destruct H as [[thread' POi' PIi' GIi'] [HLPR_RESTR BAR]].
+        apply seq_eqv_lr in BAR. destruct BAR as [TIDx [BAR TIDy]].
+        destruct BAR as [GOi' [[OEXEC' SBL'] REL'xy]].
+        red in SBL'. apply sbl_ext_TMP in SBL'. 
+        red in HLPR_RESTR. desc. simpl in *.
+        cut (graphs_sim_weak SGO GOi').
+        { ins. red in H.
+          specialize (REL_EQ_IF_GSW _ H). 
+          desc.
+          apply (RWO_RESTR_IF_SBL _ _ SBL).
+          apply (same_relation_exp REL_EQ_IF_GSW). auto. }
+        cut (graphs_sim_weak GIi GIi').
+        { ins.
+          red in SBL'. desc. 
+          eapply sbl_sim_rect; vauto.
+          { red in SBL. desc. vauto. }
+          eapply wf_tre_intra_E; vauto. }
+        eapply tre_sim_weak; vauto. 
+        replace thread' with (tid x) in *; [congruence| ]. 
+        rewrite (same_relation_exp (RWO_RESTR_IF_SBL _ _ SBL')) in REL'xy.
+        red in REL'xy. desc.
+        rewrite (same_relation_exp (TID_RESTR_IF_TRE _ _ _ RESTR')) in REL'xy. 
+        apply seq_eqv_lr in REL'xy. desc. vauto. }
+    }
+    assert (E SGO ≡₁ E GOi) as E_EQUIV. 
+    { symmetry. 
+      rewrite tr_acts_set; eauto. subst GO. unfold acts_set at 1. simpl.
+      arewrite ((fun x : actid => In x (GO_actsset ++ GO_initset)) ∩₁ Tid_ tid ≡₁ ((fun x : actid => In x (GO_actsset))  ∩₁ Tid_ tid)).
+      { rewrite IN_SET_UNION. rewrite set_inter_union_l.
+        arewrite ((fun x : actid => In x GO_initset) ∩₁ Tid_ tid ≡₁ ∅); [| basic_solver].
+        split; [| basic_solver]. red. ins. red in H. desc.
+        subst. apply INIT_GO in H. red in H. desc. destruct x; vauto.
+        red. apply programs_without_tid_init. apply find_iff_in. vauto. }
+      arewrite ((fun x : actid => In x GO_actsset) ≡₁ all_acts).
+      { apply set_equiv_exp_iff. ins. symmetry. vauto. }
+      unfold all_acts.
+      rewrite <- set_bunion_inter_compat_r.
+      unfold set_inter.
+      arewrite ((⋃₁x ∈ hlpr_restr,
+                 fun x0 =>
+                   (exists GOi0, hlpr_GO GOi0 x /\ E GOi0 x0) /\
+                   Events.tid x0 = tid)
+                  ≡₁ (⋃₁x ∈ hlpr_restr,
+                      fun x0 =>
+                        (exists GOi0, hlpr_GO GOi0 x /\ E GOi0 x0 /\
+                                 Events.tid x0 = tid))) by basic_solver 100.
+      apply set_equiv_exp_iff. ins. red. split.
+      2: { ins. red. exists ({| htid := tid; hPO := POi; hPI := PIi; hSGI := GIi |}).
+           splits; vauto.
+           exists SGO. splits; vauto.
+           { red in SBL. desc. vauto. }
+           red in SBL. desc.
+           rewrite (set_equiv_exp RESTR_EVENTS) in H.
+           red in H. desc.
+           destruct RESTR0. rewrite (set_equiv_exp tr_acts_set) in H.
+           red in H. desc. auto. }             
+      intros EGOx. cut (E SGO x); [ins; vauto| ].
+      red in EGOx.
+      destruct EGOx as [[thread' POi' PIi' GIi'] [HLPR_RESTR [GOi' [HLPR_GO [EGOi'x TIDx]]]]]. 
+      destruct x.
+      { simpl in *. exfalso.
+        apply programs_without_tid_init. apply find_iff_in. vauto. }
+      simpl in *. subst tid. 
+      red in HLPR_RESTR. red in HLPR_GO. desc. simpl in *. 
+      red in SBL'. desc. 
+      assert (thread' = thread).
+      { rewrite (set_equiv_exp RESTR_EVENTS) in EGOi'x. 
+        red in EGOi'x. desc.
+        destruct RESTR'. rewrite (set_equiv_exp tr_acts_set) in EGOi'x.
+        red in EGOi'x. desc. vauto. }
+      subst thread'. assert (PIi' = PIi /\ POi' = POi) by (split; congruence).
+      desc. subst PIi' POi'. clear THREADI' THREADO'. 
+      cut (graphs_sim_weak SGO GOi').
+      { ins. red in H. desc. apply H. auto. }
+      cut (graphs_sim_weak GIi GIi').
+      { ins.
+        red in SBL. desc. 
+        eapply sbl_sim_rect; vauto.
+        eapply wf_tre_intra_E; vauto. }
+      eapply tre_sim_weak; vauto. }      
+    red. splits; auto. 
+    { intros e ESGOx.
+      red in SBL. desc. rewrite SAME_LAB; auto.
+      destruct RESTR. rewrite tr_lab; [| by apply E_EQUIV].
+      subst GO. simpl in *.
+      destruct RESTR0. apply tr_lab0.
+      rewrite (set_equiv_exp RESTR_EVENTS) in ESGOx. red in ESGOx. desc. auto. }
+    all: by apply INTRA_REL_HELPER; vauto; ins; destruct H; desc; vauto.
+  Qed. 
+
+
+End BUILD_OMM_GRAPH. 
