src/ocamlmm/Utils.v
@@ -1,4 +1,5 @@
 Require Import Classical Peano_dec.
+From PromisingLib Require Import Basic Loc.
 From hahn Require Import Hahn.
 Set Implicit Arguments.
 
@@ -48,6 +49,150 @@ Proof.
   ins. red. split.
   all: red; ins; apply H; auto.
 Qed. 
+
+Lemma seq_eqv_lr_l {A: Type} (d1 d2: A -> Prop) r:
+  r ≡ ⦗d1⦘ ⨾ r ⨾ ⦗d2⦘ -> r ≡ ⦗d1⦘ ⨾ r.
+Proof. ins. rewrite H. basic_solver. Qed. 
+
+Lemma seq_eqv_lr_r {A: Type} (d1 d2: A -> Prop) r:
+  r ≡ ⦗d1⦘ ⨾ r ⨾ ⦗d2⦘ -> r ≡ r ⨾ ⦗d2⦘.
+Proof. ins. rewrite H. basic_solver. Qed.
+
+Lemma inter_subset_helper {A: Type} (S S1 S2: A -> Prop):
+  (forall x (Sx: S x), S1 x <-> S2 x) -> S ∩₁ S1 ≡₁ S ∩₁ S2.
+Proof.
+  ins. apply set_equiv_exp_iff. ins. specialize (H x).
+  unfold set_inter. 
+  split; ins; desc; split; intuition.
+Qed.
+
+Lemma set_finite_alt {A: Type} (S: A -> Prop) (FIN: set_finite S):
+  exists findom, forall x, S x <-> In x findom.
+Proof.
+  destruct FIN as [lst FIN].
+  exists (filterP S lst). ins. split.
+  { ins. apply in_filterP_iff. split; auto. }
+  ins. apply in_filterP_iff in H. desc. auto. 
+Qed.
+
+Lemma bunion_more_alt: forall {A B : Type} (x y : A -> Prop),
+    x ≡₁ y ->
+    forall (x0 y0 : A -> relation B), (forall a, x0 a ≡ y0 a) -> (⋃x ∈ x, x0 x) ≡ (⋃x ∈ y, y0 x).
+Proof.
+  ins. apply same_relation_exp_iff. ins. red. splits.
+  { unfold bunion. ins. desc. exists a. splits.
+    { apply H. auto. }
+    apply H0. auto. }
+  { unfold bunion. ins. desc. exists a. splits. 
+    { apply H. auto. }
+    apply H0. auto. }
+Qed.
+
+    
+Lemma IN_SET_UNION {A: Type} (l1 l2: list A):
+  (fun x => In x (l1 ++ l2)) ≡₁ (fun x => In x l1) ∪₁ (fun x => In x l2).
+Proof. 
+  ins. apply set_equiv_exp_iff. ins. split.
+  { ins. red. apply in_app_or. auto. }
+  ins. red in H. apply in_or_app. auto.
+Qed.
+
+Lemma eqv_rel_more_inv {A: Type} (S1 S2: A -> Prop) (EQV_REL: ⦗S1⦘ ≡ ⦗S2⦘):
+  S1 ≡₁ S2.
+Proof. 
+  apply set_equiv_exp_iff. ins.
+  apply (same_relation_exp) with (x := x) (y := x) in EQV_REL.
+  unfold eqv_rel in EQV_REL. red in EQV_REL. desc. 
+  red. splits; desc; intuition.
+Qed.
+
+Lemma unique_restr {A: Type} x y (r: relation A) (Rxy: r x y):
+  ⦗eq x⦘ ⨾ r ⨾ ⦗eq y⦘ ≡ singl_rel x y.
+Proof.
+  ins. rewrite seq_eqv_lr. split.
+  { red. ins. desc. red. splits; auto. }
+  red. ins. red in H. desc. splits; vauto.
+Qed.
+
+Lemma singl_rel_restr {A: Type} (x y: A):
+  singl_rel x y ≡ ⦗eq x⦘ ⨾ singl_rel x y ⨾ ⦗eq y⦘. 
+Proof. ins. basic_solver. Qed. 
+
+Lemma rel_endpoints_dom {A: Type} (D C EL ER : A -> Prop) r (DOM: r ≡ ⦗D⦘ ⨾ r ⨾ ⦗C⦘):
+  ⦗EL⦘ ⨾ r ⨾ ⦗ER⦘ ≡ ⦗EL ∩₁ D⦘ ⨾ r ⨾ ⦗ER ∩₁ C⦘.
+Proof.
+  rewrite set_interC with (s' := C). 
+  do 2 rewrite id_inter. rewrite !seqA.
+  seq_rewrite <- DOM. basic_solver.
+Qed.
+
+Lemma seq_compl_helper {A: Type} (r: relation A) (S: A -> Prop):
+  r ⨾ ⦗set_compl S⦘ ≡ r \ set_full × S.
+Proof.
+  rewrite <- (seq_id_l r) at 1.
+  rewrite seqA. 
+  pose proof (seq_eqv_lr r (fun _ : A => True) (set_compl S)).
+  seq_rewrite H. 
+  apply same_relation_exp_iff. ins.
+  split.
+  { ins. desc. red. splits; auto. red. basic_solver. }
+  ins. red in H0. desc. splits; auto.
+  red. red. red in H1. 
+  ins. apply H1. unfold cross_rel. split; basic_solver. 
+Qed. 
+
+Lemma MINUS_DISTR_L {A: Type} (r: relation A) (S1 S2: A -> Prop):
+  ⦗S1 \₁ S2⦘ ⨾ r ≡ ⦗S1⦘ ⨾ r \ ⦗S2⦘ ⨾ r.
+Proof. 
+  ins. red. split; [| basic_solver].
+  red. ins. red. apply seq_eqv_l in H. desc.
+  red in H. desc.
+  split; [basic_solver |].
+  red. ins. apply seq_eqv_l in H2. basic_solver.
+Qed. 
+
+Lemma MINUS_DISTR_R {A: Type} (r: relation A) (S1 S2: A -> Prop):
+  r ⨾ ⦗S1 \₁ S2⦘ ≡ r ⨾ ⦗S1⦘ \ r ⨾ ⦗S2⦘.
+Proof. 
+  ins. red. split; [| basic_solver].            
+  red. ins. red. apply seq_eqv_r in H. desc.
+  red in H0. desc.
+  split; [basic_solver |].
+  red. ins. apply seq_eqv_r in H2. basic_solver.
+Qed. 
+
+Lemma MINUS_GROUP {A: Type} (r1 r2 r3: relation A):
+  (r1 \ r2) \ r3 ≡ r1 \ (r2 ∪ r3).
+Proof. 
+  ins. red. split; [| basic_solver].
+  red. ins. red. red in H. desc. red in H. desc.
+  split; auto. red. ins. red in H2. basic_solver.
+Qed.
+
+Lemma SUPSET_RESTR {A: Type} (r1 r2: relation A) S (INCL: r1 ⊆ r2) (RESTR: r2 ≡ ⦗S⦘ ⨾ r2 ⨾ ⦗S⦘):
+  r1 ≡ ⦗S⦘ ⨾ r1 ⨾ ⦗S⦘. 
+Proof.
+  ins. split; [| basic_solver].
+  red. ins. apply seq_eqv_lr.
+  red in RESTR. desc. red in RESTR.
+  red in INCL. 
+  pose proof (INCL x y H) as R2.
+  specialize (RESTR x y R2). apply seq_eqv_lr in RESTR. desc.
+  splits; auto.
+Qed.
+
+Lemma RESTR_SEQ  {A: Type} (r1 r2: relation A) (D: A -> Prop):
+  restr_rel D r1 ⨾ restr_rel D r2 ⊆ restr_rel D (r1 ⨾ r2). 
+Proof. ins. basic_solver. Qed.
+
+
+Lemma find_iff_in {A: Type} (M: IdentMap.t A) k: 
+  IdentMap.In k M <-> exists elt, Some elt = IdentMap.find k M. 
+Proof.
+  pose proof (@UsualFMapPositive.UsualPositiveMap.Facts.in_find_iff _ M k).
+  pose proof OPT_VAL (IdentMap.find k M).
+  eapply iff_stepl; [eapply H0 | symmetry; eauto]. 
+Qed.
 
 Ltac remove_emptiness :=
   repeat (rewrite set_inter_empty_r || rewrite set_inter_empty_l ||
